code/aes-gcm/Hacl.AES_256_GCM.M32.fst
@@ -21,7 +21,7 @@ type aes_gcm_ctx = lbuffer uint64 aes_gcm_ctx_len
 val aes256_gcm_init:
     ctx: aes_gcm_ctx
   -> key: lbuffer uint8 32ul
-  -> nonce: lbuffer uint8 16ul ->
+  -> nonce: lbuffer uint8 12ul ->
   Stack unit
   (requires (fun h -> live h ctx /\ live h key /\ live h nonce))
   (ensures (fun h0 _ h1 -> modifies1 ctx h0 h1))
@@ -30,13 +30,13 @@ let aes256_gcm_init ctx key nonce =
   push_frame();
   let gcm_key = create 16ul (u8 0) in
   let tag_mix = create 16ul (u8 0) in
-  let nonce0 = create 16ul (u8 0) in
+  let nonce0 = create 12ul (u8 0) in
   let aes_ctx = sub ctx (size 0) (size 128) in
   let gcm_ctx = sub ctx (size 128) (size 266) in
   aes256_init aes_ctx key nonce0;
-  aes256_key_block gcm_key aes_ctx;
+  aes256_key_block gcm_key aes_ctx (size 0);
   aes256_set_nonce aes_ctx nonce;
-  aes256_key_block tag_mix aes_ctx;
+  aes256_key_block tag_mix aes_ctx (size 1);
   gcm_init gcm_ctx gcm_key;
   ctx.(394ul) <- uint_from_bytes_le #U64 (sub tag_mix 0ul 8ul);
   ctx.(395ul) <- uint_from_bytes_le #U64 (sub tag_mix 8ul 8ul);
@@ -67,7 +67,7 @@ let aes256_gcm_encrypt ctx len out text aad_len aad =
   let aes_ctx = sub ctx (size 0) (size 128) in
   let gcm_ctx = sub ctx (size 128) (size 266) in
   let tag_mix = sub ctx (size 394) (size 2) in
-  aes256_ctr len cip text aes_ctx;
+  aes256_ctr len cip text aes_ctx (size 2);
   gcm_update_blocks_padded gcm_ctx aad_len aad;
   gcm_update_blocks_padded gcm_ctx len cip;
   uint_to_bytes_be #U64 (sub tmp (size 0) (size 8)) (to_u64 (aad_len *. 8ul));
@@ -134,7 +134,7 @@ let aes256_gcm_decrypt ctx len out cipher aad_len aad =
   let res8 = result.(0ul) in
   let r =
     if Lib.RawIntTypes.u8_to_UInt8 res8 = 0uy then (
-      aes256_ctr len out ciphertext aes_ctx;
+      aes256_ctr len out ciphertext aes_ctx (size 2);
       true)
     else (
       let h9 = ST.get () in
