code/aes/Hacl.AES_128.BitSlice.fst
@@ -26,7 +26,7 @@ let create_ctx () = create_ctx M32 Spec.AES.AES128
 val aes128_init:
     ctx: aes_ctx
   -> key: skey
-  -> nonce: lbuffer uint8 16ul ->
+  -> nonce: lbuffer uint8 12ul ->
   Stack unit
   (requires (fun h -> live h ctx /\ live h nonce /\ live h key))
   (ensures  (fun h0 _ h1 -> modifies1 ctx h0 h1))
@@ -38,7 +38,7 @@ let aes128_init ctx key nonce = aes128_bitslice_init ctx key nonce
 [@ CInline ]
 val aes128_set_nonce:
     ctx: aes_ctx
-  -> nonce: lbuffer uint8 16ul ->
+  -> nonce: lbuffer uint8 12ul ->
   Stack unit
   (requires (fun h -> live h ctx /\ live h nonce))
   (ensures  (fun h0 _ h1 -> modifies1 ctx h0 h1))
@@ -50,13 +50,14 @@ let aes128_set_nonce ctx nonce = aes_set_nonce ctx nonce
 [@ CInline ]
 val aes128_key_block:
     kb: lbuffer uint8 16ul
-  -> ctx:aes_ctx ->
+  -> ctx:aes_ctx
+  -> counter:size_t ->
   Stack unit
   (requires (fun h -> live h kb /\ live h ctx))
   (ensures  (fun h0 _ h1 -> modifies1 kb h0 h1))
 
 [@ CInline ]
-let aes128_key_block kb ctx = aes_key_block #M32 #Spec.AES.AES128 kb ctx
+let aes128_key_block kb ctx counter = aes_key_block #M32 #Spec.AES.AES128 kb ctx counter
 
 
 inline_for_extraction noextract
@@ -77,11 +78,12 @@ val aes128_ctr:
   -> out: lbuffer uint8 len
   -> inp: lbuffer uint8 len
   -> ctx: aes_ctx
+  -> counter: size_t
   -> ST unit
   (requires (fun h -> live h out /\ live h inp /\ live h ctx))
   (ensures (fun h0 _ h1 -> modifies (loc out) h0 h1))
 
-let aes128_ctr len out inp ctx = aes_ctr #M32 #Spec.AES.AES128 len out inp ctx
+let aes128_ctr len out inp ctx c = aes_ctr #M32 #Spec.AES.AES128 len out inp ctx c
 
 
 [@ CInline ]
@@ -90,12 +92,13 @@ val aes128_ctr_encrypt:
   -> out: lbuffer uint8 len
   -> inp: lbuffer uint8 len
   -> k:skey
-  -> n:lbuffer uint8 16ul
+  -> n:lbuffer uint8 12ul
+  -> counter:size_t
   -> ST unit
   (requires (fun h -> live h out /\ live h inp /\ live h k /\ live h n))
   (ensures (fun h0 _ h1 -> modifies (loc out) h0 h1))
 
-let aes128_ctr_encrypt len out inp k n = aes_ctr_encrypt #M32 #Spec.AES.AES128 len out inp k n
+let aes128_ctr_encrypt len out inp k n c = aes_ctr_encrypt #M32 #Spec.AES.AES128 len out inp k n c
 
 
 [@ CInline ]
@@ -104,8 +107,9 @@ val aes128_ctr_decrypt:
   -> out: lbuffer uint8 len
   -> inp: lbuffer uint8 len
   -> k:skey
-  -> n:lbuffer uint8 16ul
+  -> n:lbuffer uint8 12ul
+  -> counter:size_t
   -> ST unit
   (requires (fun h -> live h out /\ live h inp /\ live h k /\ live h n))
   (ensures (fun h0 _ h1 -> modifies (loc out) h0 h1))
-let aes128_ctr_decrypt len out inp k n = aes_ctr_decrypt #M32 #Spec.AES.AES128 len out inp k n
+let aes128_ctr_decrypt len out inp k n c = aes_ctr_decrypt #M32 #Spec.AES.AES128 len out inp k n c
