code/aes/Hacl.AES_256.NI.fst
@@ -26,7 +26,7 @@ let create_ctx () = create_ctx MAES Spec.AES.AES256
 val aes256_init:
     ctx: aes_ctx
   -> key: skey 
-  -> nonce: lbuffer uint8 16ul ->
+  -> nonce: lbuffer uint8 12ul ->
   Stack unit
   (requires (fun h -> live h ctx /\ live h nonce /\ live h key))
   (ensures  (fun h0 _ h1 -> modifies1 ctx h0 h1))
@@ -52,7 +52,7 @@ let aes256_encrypt_block ob ctx ib =
 [@ CInline ]
 val aes256_set_nonce:
     ctx: aes_ctx
-  -> nonce: lbuffer uint8 16ul ->
+  -> nonce: lbuffer uint8 12ul ->
   Stack unit
   (requires (fun h -> live h ctx /\ live h nonce))
   (ensures  (fun h0 _ h1 -> modifies1 ctx h0 h1))
@@ -64,13 +64,14 @@ let aes256_set_nonce ctx nonce = aes_set_nonce ctx nonce
 [@ CInline ]
 val aes256_key_block:
     kb: lbuffer uint8 16ul
-  -> ctx:aes_ctx ->
+  -> ctx:aes_ctx
+  -> counter:size_t ->
   Stack unit
   (requires (fun h -> live h kb /\ live h ctx))
   (ensures  (fun h0 _ h1 -> modifies1 kb h0 h1))
 
 [@ CInline ]
-let aes256_key_block kb ctx = aes_key_block #MAES #Spec.AES.AES256 kb ctx
+let aes256_key_block kb ctx counter = aes_key_block #MAES #Spec.AES.AES256 kb ctx counter
 
 
 inline_for_extraction noextract
@@ -92,11 +93,12 @@ val aes256_ctr:
   -> out: lbuffer uint8 len
   -> inp: lbuffer uint8 len
   -> ctx: aes_ctx
+  -> counter: size_t
   -> ST unit
   (requires (fun h -> live h out /\ live h inp /\ live h ctx))
   (ensures (fun h0 _ h1 -> modifies (loc out) h0 h1))
 
-let aes256_ctr len out inp ctx =  aes_ctr #MAES #Spec.AES.AES256 len out inp ctx
+let aes256_ctr len out inp ctx c =  aes_ctr #MAES #Spec.AES.AES256 len out inp ctx c
 
 
 
@@ -106,12 +108,13 @@ val aes256_ctr_encrypt:
   -> out: lbuffer uint8 len
   -> inp: lbuffer uint8 len
   -> k:skey
-  -> n:lbuffer uint8 16ul
+  -> n:lbuffer uint8 12ul
+  -> counter:size_t
   -> ST unit
   (requires (fun h -> live h out /\ live h inp /\ live h k /\ live h n))
   (ensures (fun h0 _ h1 -> modifies (loc out) h0 h1))
 
-let aes256_ctr_encrypt len out inp k n = aes_ctr_encrypt #MAES #Spec.AES.AES256 len out inp k n
+let aes256_ctr_encrypt len out inp k n c = aes_ctr_encrypt #MAES #Spec.AES.AES256 len out inp k n c
 
 
 [@ CInline ]
@@ -120,8 +123,9 @@ val aes256_ctr_decrypt:
   -> out: lbuffer uint8 len
   -> inp: lbuffer uint8 len
   -> k:skey
-  -> n:lbuffer uint8 16ul
+  -> n:lbuffer uint8 12ul
+  -> counter:size_t
   -> ST unit
   (requires (fun h -> live h out /\ live h inp /\ live h k /\ live h n))
   (ensures (fun h0 _ h1 -> modifies (loc out) h0 h1))
-let aes256_ctr_decrypt len out inp k n = aes_ctr_decrypt #MAES #Spec.AES.AES256 len out inp k n
+let aes256_ctr_decrypt len out inp k n c = aes_ctr_decrypt #MAES #Spec.AES.AES256 len out inp k n c
